feat(library/init/meta): corec_on for coinductive predicates

library/init/meta/coinductive_predicates.lean
@@ -65,6 +65,39 @@ meta def add_theorem_by (n : name) (ls : list name) (type : expr) (locals : list
 meta def is_assigned (m : expr): tactic bool :=
 ((get_assignment m >> return ff) <|> return tt)
 
+meta def mk_exists_lst (args : list expr) (inner : expr) : tactic expr :=
+args.mfoldr (λarg i:expr, do
+    sort l ← infer_type arg.local_type,
+    return $ (const `Exists [l] : expr) arg.local_type (i.lambdas [arg]))
+  inner
+
+meta def mk_op_lst (op : expr) (empty : expr) : list expr → expr
+| []         := empty
+| (hd :: tl) := tl.foldr (λa c, op a c) hd
+
+meta def mk_and_lst : list expr → expr := mk_op_lst `(and) `(true)
+
+meta def mk_or_lst : list expr → expr := mk_op_lst `(or) `(false)
+
+meta def elim_gen_prod : nat → expr → list expr → tactic (list expr × expr)
+| 0       e hs := return (hs, e)
+| (n + 1) e hs := do
+  [([h, h'], _)] ← induction e [],
+  elim_gen_prod n h' (hs ++ [h])
+
+private meta def elim_gen_sum_aux : nat → expr → list expr → tactic (list expr × expr)
+| 0       e hs := return (hs, e)
+| (n + 1) e hs := do
+  [([h], _), ([h'], _)] ← induction e [],
+  swap,
+  elim_gen_sum_aux n h (h'::hs)
+
+meta def elim_gen_sum (n : nat) (e : expr) : tactic (list expr) := do
+  (hs, h') ← elim_gen_sum_aux n e [],
+  gs ← get_goals,
+  set_goals ((gs.taken n).reverse ++ gs.dropn n),
+  return $ hs.reverse ++ [h']
+
 /-
 The coinductive predicate `pred`:
 
@@ -86,148 +119,161 @@ where
   | r : ∀a [f], b[pred/pred'] → pred.functional a [f] p
 
   lemma {u} pred.functional.mono (A) ([pred₁] [pred₂] : a → Prop) [(h : ∀b, pred₁ b → pred₂ b)] :
-    ∀p, pred.functional A pred₁ p → pred.functional A pred₂ p :=
-  pred.functional.rec A f (pred.functional A f')
-    (take p, pred.functional.r A f' p[mono with h])
+    ∀p, pred.functional A pred₁ p → pred.functional A pred₂ p
 
   def {u} pred_i (A) (a) : Prop :=
   ∃[pred'], (Λi, ∀a, pred_i a → pred_i.functional A [pred] a) ∧ pred'_i a
 
   lemma {u} pred_i.corec_functional (A) [Λi, C_i : a_i → Prop] [Λi, h : ∀a, C_i a → pred_i.functional A C_i a] :
-    ∀a, C_i a → pred_i A a :=
-  take a ha, ⟨[C], [h], ha⟩
+    ∀a, C_i a → pred_i A a
 
-  lemma {u} pred_i.destruct (A) (a) : pred A a → pred.functional A [pred A] a :=
-  Exists.rec (a → Prop) (λf, (∀a, f a → pred.functional A f a) ∧ f a)
-    (pred.functional A (pred A a) a) h $
-  take f, and.rec.{0} (∀a, f a → pred.functional A f a) (f a) $
-    assume h₁ : ∀a, f a → pred.functional A f a, assume h₂ : f a,
-    pred.functional.mono A f (pred A) (pred.corec_functional A f h₁) a (h₁ a h₂))
+  lemma {u} pred_i.destruct (A) (a) : pred A a → pred.functional A [pred A] a
 
-  lemma {u} pred_i.construct (A) : ∀a, pred_i.functional A [pred A] a → pred_i A a :=
-  pred.corec_functional A (pred.functional A (pred A))
-    (pred.functional.mono A (pred A) (pred.functional A (pred A)) (pred.destruct A))
+  lemma {u} pred_i.construct (A) : ∀a, pred_i.functional A [pred A] a → pred_i A a
 
   lemma {u} pred_i.cases_on (A) (C : a → Prop) {a} (h : pred_i a) [Λi, ∀a, b → C p] → C a
 
-  -- TODO:
   lemma {u} pred_i.corec_on (A) [(C : a → Prop)] (a) (h : C_i a)
-    [Λi, h_i : ∀a, C_i a → [V j ∃b, a = p]] :
-    pred_i A a
+    [Λi, h_i : ∀a, C_i a → [V j ∃b, a = p]] : pred_i A a
 
-  lemma {u} pred.r (A) (b) : pred_i A p :=
-  pred_i.construct A p $ pred_i.functional.r A [pred A] b
+  lemma {u} pred.r (A) (b) : pred_i A p
 -/
 
 open level expr tactic
 
 namespace add_coinductive_predicate
 
-/- private -/ meta structure pred_predata : Type :=
+/- private -/ meta structure coind_rule : Type :=
+(orig_nm  : name)
+(func_nm  : name)
+(type     : expr)
+(loc_type : expr)
+(args     : list expr)
+(loc_args : list expr)
+(concl    : expr)
+(insts    : list expr)
+
+/- private -/ meta structure coind_pred : Type :=
 (u_names  : list name)
 (params   : list expr)
 (pd_name  : name)
-(pred     : expr)
 (type     : expr)
-(intros   : list (name × expr))
+(intros   : list coind_rule)
 (locals   : list expr)
 (f₁ f₂    : expr)
 (u_f      : level)
-(func     : expr)
 
-namespace pred_predata
+namespace coind_pred
 
-meta def u_params (pd : pred_predata) : list level :=
+meta def u_params (pd : coind_pred) : list level :=
 pd.u_names.map param
 
-meta def f₁_l (pd : pred_predata) : expr :=
+meta def f₁_l (pd : coind_pred) : expr :=
 pd.f₁.app_of_list pd.locals
 
-meta def f₂_l (pd : pred_predata) : expr :=
+meta def f₂_l (pd : coind_pred) : expr :=
 pd.f₂.app_of_list pd.locals
 
-meta def func_g (pd : pred_predata) : expr :=
+meta def pred (pd : coind_pred) : expr :=
+const pd.pd_name pd.u_params
+
+meta def func (pd : coind_pred) : expr :=
+const (pd.pd_name ++ "functional") pd.u_params
+
+meta def func_g (pd : coind_pred) : expr :=
 pd.func.app_of_list $ pd.params
 
-meta def pred_g (pd : pred_predata) : expr :=
+meta def pred_g (pd : coind_pred) : expr :=
 pd.pred.app_of_list $ pd.params
 
-meta def impl_locals (pd : pred_predata) : list expr :=
+meta def impl_locals (pd : coind_pred) : list expr :=
 pd.locals.map to_implicit_binder
 
-meta def impl_params (pd : pred_predata) : list expr :=
+meta def impl_params (pd : coind_pred) : list expr :=
 pd.params.map to_implicit_binder
 
-meta def le (pd : pred_predata) (f₁ f₂ : expr) : expr :=
+meta def le (pd : coind_pred) (f₁ f₂ : expr) : expr :=
 (imp (f₁.app_of_list pd.locals) (f₂.app_of_list pd.locals)).pis pd.impl_locals
 
-meta def corec (pd : pred_predata) : expr :=
-const (pd.pd_name ++ "corec_functional") pd.u_params
+meta def corec_functional (pd : coind_pred) : expr :=
+(const (pd.pd_name ++ "corec_functional") pd.u_params).app_of_list pd.params
 
-meta def mono (pd : pred_predata) : expr :=
-const (pd.func.const_name ++ "mono") pd.u_params
+meta def mono (pd : coind_pred) : expr :=
+(const (pd.func.const_name ++ "mono") pd.u_params).app_of_list pd.params
 
-meta def rec' (pd : pred_predata) : tactic expr :=
+meta def rec' (pd : coind_pred) : tactic expr :=
 mk_const (pd.func.const_name ++ "rec")
   -- ^^ `rec`'s universes are not always `u_params`, e.g. eq, wf, false
 
-meta def construct (pd : pred_predata) : expr :=
-const (pd.pd_name ++ "construct") pd.u_params
+meta def construct (pd : coind_pred) : expr :=
+(const (pd.pd_name ++ "construct") pd.u_params).app_of_list pd.params
 
-meta def destruct (pd : pred_predata) : expr :=
-const (pd.pd_name ++ "destruct") pd.u_params
+meta def destruct (pd : coind_pred) : expr :=
+(const (pd.pd_name ++ "destruct") pd.u_params).app_of_list pd.params
 
-meta def add_theorem (pd : pred_predata) (n : name) (type : expr) (locals : list expr) (tac : tactic unit) :
+meta def add_theorem (pd : coind_pred) (n : name) (type : expr) (locals : list expr) (tac : tactic unit) :
   tactic expr :=
 add_theorem_by n pd.u_names type (pd.impl_params ++ locals) tac
 
-end pred_predata
+end coind_pred
 
 end add_coinductive_predicate
 
 open add_coinductive_predicate
 
 meta def add_coinductive_predicate
-  (u_params : list name) (params : list expr) (preds : list $ expr × list expr) : command := do
+  (u_names : list name) (params : list expr) (preds : list $ expr × list expr) : command := do
   let params_names := params.map local_pp_name,
-  let u_params' := u_params.map param,
+  let u_params := u_names.map param,
 
-  pds ← preds.mmap (λ⟨c, is⟩, do
+  pre_info ← preds.mmap (λ⟨c, is⟩, do
     (ls, `(Prop)) ← mk_local_pis c.local_type,
     let n := if preds.length = 1 then "" else "_" ++ c.local_pp_name.last_string,
     f₁ ← mk_local_def (mk_simple_name $ "C" ++ n) c.local_type,
     f₂ ← mk_local_def (mk_simple_name $ "C₂" ++ n) c.local_type,
-    sort u_f ← infer_type f₁ >>= infer_type,
-    let func : expr := const (c.local_uniq_name ++ "functional") u_params',
-    return {tactic.add_coinductive_predicate.pred_predata .
-      pd_name := c.local_uniq_name,
-      pred := const c.local_uniq_name u_params', type := c.local_type,
-      intros := is.map (λi, (i.local_uniq_name, i.local_type)),
-      locals := ls, params := params, u_names := u_params,
-      f₁ := f₁, f₂ := f₂, u_f := u_f, func := func}),
+    return (ls, (f₁, f₂))),
 
-  let f₁ := pds.map pred_predata.f₁,
-  let f₂ := pds.map pred_predata.f₂,
+  let fs := pre_info.map prod.snd,
+  let fs₁ := fs.map prod.fst,
+  let fs₂ := fs.map prod.snd,
+
+  pds ← (preds.zip pre_info).mmap (λ⟨⟨c, is⟩, ls, f₁, f₂⟩, do
+    sort u_f ← infer_type f₁ >>= infer_type,
+    let pred_g := λc:expr, (const c.local_uniq_name u_params : expr).app_of_list params,
+    intros ← is.mmap (λi, do
+      (args, t') ← mk_local_pis i.local_type,
+      (name.mk_string sub p) ← return i.local_uniq_name,
+      let loc_args := args.map $ λe, (fs₁.zip preds).foldl (λ(e:expr) ⟨f, c, _⟩, 
+        e.replace_with (pred_g c) f) e,
+      let t' := t'.replace_with (pred_g c) f₂,
+      return { tactic.add_coinductive_predicate.coind_rule .
+        orig_nm  := i.local_uniq_name,
+        func_nm  := (p ++ "functional") ++ sub,
+        type     := i.local_type,
+        loc_type := t'.pis loc_args,
+        concl    := t',
+        loc_args := loc_args,
+        args     := args,
+        insts    := t'.get_app_args }),
+    return { tactic.add_coinductive_predicate.coind_pred .
+      pd_name := c.local_uniq_name, type := c.local_type, f₁ := f₁, f₂ := f₂, u_f := u_f,
+      intros := intros, locals := ls, params := params, u_names := u_names }),
 
   /- Introduce all functionals -/
-  pds.mmap (λpd:pred_predata, do
-    let func_f₁ := pd.func_g.app_of_list $ f₁,
-    let func_f₂ := pd.func_g.app_of_list $ f₂,
+  pds.mmap (λpd:coind_pred, do
+    let func_f₁ := pd.func_g.app_of_list $ fs₁,
+    let func_f₂ := pd.func_g.app_of_list $ fs₂,
 
     /- Define functional for `pd` as inductive predicate -/
-    func_intros ← pd.intros.mmap (λ⟨nr, t⟩, do
-      (bs, t') ← mk_local_pis t,
-      (name.mk_string sub p) ← return $ nr,
-      let bs := bs.map $ λe, pds.foldl (λ(e:expr) (pd:pred_predata),
-        e.replace_with pd.pred_g pd.f₁) e,
-      let t' := t'.replace_with pd.pred_g (pd.func_g.app_of_list $ f₁),
-      return ((p ++ "functional") ++ sub, t'.pis $ params ++ f₁ ++ bs)),
-    let func_type := pd.type.pis $ params ++ f₁,
-    add_inductive pd.func.const_name u_params (params.length + preds.length) func_type func_intros,
+    func_intros ← pd.intros.mmap (λr:coind_rule, do
+      let t := instantiate_local pd.f₂.local_uniq_name (pd.func_g.app_of_list fs₁) r.loc_type,
+      return (r.func_nm, t.pis $ params ++ fs₁)),
+    add_inductive pd.func.const_name u_names
+      (params.length + preds.length) (pd.type.pis $ params ++ fs₁) func_intros,
 
     /- Prove monotonicity rule -/
     let mono_type :=
-      pds.reverse.foldl (λc (pd:pred_predata), ((pd.le pd.f₁ pd.f₂).imp c).pis [pd.f₁, pd.f₂]) $
+      pds.reverse.foldl (λc (pd:coind_pred), ((pd.le pd.f₁ pd.f₂).imp c).pis [pd.f₁, pd.f₂]) $
       pd.le func_f₁ func_f₂,
     pd.add_theorem (pd.func.const_name ++ "mono") mono_type [] (do
       hf ← pds.mmap (λpd, do
@@ -239,12 +285,12 @@ meta def add_coinductive_predicate
       apply $ m.app_of_list params, -- somehow `induction` / `cases` doesn't work?
       focus $ func_intros.map (λ⟨n, t⟩, do
         bs ← intros,
-        ms ← apply_core ((const n u_params').app_of_list $ params ++ fs₂) { all := tt },
+        ms ← apply_core ((const n u_params).app_of_list $ params ++ fs₂) { all := tt },
         params ← (ms.zip bs).mfilter (λ⟨m, d⟩, is_assigned m),
         focus $ params.map (λ⟨m, d⟩, apply d <|> first (hfs.map $ λ hf, apply hf >> apply d))))),
 
-  pds.mmap (λpd:pred_predata, do
-    let func_f := λpd:pred_predata, pd.func_g.app_of_list $ pds.map pred_predata.f₁,
+  pds.mmap (λpd:coind_pred, do
+    let func_f := λpd:coind_pred, pd.func_g.app_of_list $ pds.map coind_pred.f₁,
 
     /- define final predicate -/
     pred_body ← (do
@@ -252,85 +298,103 @@ meta def add_coinductive_predicate
         (λcont pd, to_expr ``(%%(pd.le pd.f₁ (func_f pd)) ∧ %%cont))
         (pd.f₁.app_of_list pd.locals),
       pds.reverse.mfoldl (λcont pd, to_expr ``(@Exists %%pd.type %%(cont.lambdas [pd.f₁]))) corec),
-    add_decl $ mk_definition pd.pd_name u_params (pd.type.pis $ params) $
+    add_decl $ mk_definition pd.pd_name u_names (pd.type.pis $ params) $
       pred_body.lambdas $ params ++ pd.locals,
 
     /- prove `corec_functional` rule -/
-    hs ← pds.mmap $ λpd:pred_predata, mk_local_def `hc $ pd.le pd.f₁ (func_f pd),
-    pd.add_theorem (pd.pred.const_name ++ "corec_functional") (pd.le pd.f₁ pd.pred_g) (f₁ ++ hs) (do
+    hs ← pds.mmap $ λpd:coind_pred, mk_local_def `hc $ pd.le pd.f₁ (func_f pd),
+    pd.add_theorem (pd.pred.const_name ++ "corec_functional") (pd.le pd.f₁ pd.pred_g) (fs₁ ++ hs) (do
       ls ← intro_lst $ pd.locals.map local_pp_name,
       h ← intro `h,
       whnf_target,
-      f₁.mmap existsi,
+      fs₁.mmap existsi,
       hs.mmap (λf, constructor >> exact f),
       exact h)),
- 
-  let func_f := λpd : pred_predata, pd.func_g.app_of_list $ pds.map pred_predata.pred_g,
+
+  let func_f := λpd : coind_pred, pd.func_g.app_of_list $ pds.map coind_pred.pred_g,
 
   /- prove `destruct` rules -/
-  pds.enum.mmap (λd:ℕ × pred_predata, do
-    let n := d.1,
-    let pd := d.2,
+  pds.enum.mmap (λ⟨n, pd⟩, do
     let destruct := pd.le pd.pred_g (func_f pd),
     pd.add_theorem (pd.pred.const_name ++ "destruct") destruct [] (do
       ls ← intro_lst $ pd.locals.map local_pp_name,
       h ← intro `h,
-      (fs, h) ← pds.reverse.mfoldl (λ(c:list expr × expr) (pd:pred_predata), do
-          [([f, hf], [])] ← induction c.2 [`f, `hf],
-          return (c.1 ++ [f], hf))
-        ([], h),
-      (hs, h) ← pds.reverse.mfoldl (λ(c:list expr × expr) (pd:pred_predata), do
-          [([h, h'], [])] ← induction c.2 [`h, `h'],
-          return (c.1 ++ [h], h'))
-        ([], h),
-      apply $ pd.mono.app_of_list $ params,
-      pds.mmap (λpd:pred_predata, focus1 $ do
-        apply $ pd.corec.app_of_list $ params,
+      (fs, h) ← elim_gen_prod pds.length h [],
+      (hs, h) ← elim_gen_prod pds.length h [],
+      apply $ pd.mono,
+      pds.mmap (λpd:coind_pred, focus1 $ do
+        apply $ pd.corec_functional,
         focus $ hs.map exact),
       some h' ← return $ hs.nth n,
       apply h',
       exact h)),
 
   /- prove `construct` rules -/
-  pds.mmap (λpd:pred_predata,
+  pds.mmap (λpd:coind_pred,
     pd.add_theorem (pd.pred.const_name ++ "construct") (pd.le (func_f pd) pd.pred_g) [] (do
-      let func_pred_g := λpd:pred_predata,
-        pd.func.app_of_list $ params ++ pds.map (λpd:pred_predata, pd.pred.app_of_list params),
-      apply $ pd.corec.app_of_list $ params ++ pds.map func_pred_g,
-      focus $ pds.map (λpd:pred_predata, do
-        apply $ pd.mono.app_of_list $ params,
+      let func_pred_g := λpd:coind_pred,
+        pd.func.app_of_list $ params ++ pds.map (λpd:coind_pred, pd.pred.app_of_list params),
+      apply $ pd.corec_functional.app_of_list $ pds.map func_pred_g,
+      focus $ pds.map (λpd:coind_pred, do
+        apply pd.mono,
         focus $ pds.map (λpd, apply pd.destruct)))),
 
   /- prove `cases_on` rules -/
-  pds.mmap (λpd:pred_predata, do
-    let motiv := (sort level.zero : expr).pis $ pd.locals,
-    C ← mk_local' `C binder_info.implicit motiv,
+  pds.mmap (λpd:coind_pred, do
+    let C := pd.f₁.to_implicit_binder,
     h ← mk_local_def `h $ pd.pred_g.app_of_list pd.locals,
-    rules ← pd.intros.mmap (λp:name × expr, do
-      (args, concl) ← mk_local_pis p.2,
-      mk_local_def p.1 $ (C.app_of_list $ concl.get_app_args.dropn params.length).pis args),
+    rules ← pd.intros.mmap (λr:coind_rule, do
+      mk_local_def (mk_simple_name r.orig_nm.last_string) $ (C.app_of_list r.insts).pis r.args),
     cases_on ← pd.add_theorem (pd.pred.const_name ++ "cases_on")
-      (C.app_of_list $ pd.locals) ([C] ++ pd.impl_locals ++ [h] ++ rules)
+      (C.app_of_list pd.locals) ([C] ++ pd.impl_locals ++ [h] ++ rules)
       (do
         func_rec ← pd.rec',
-        apply $ func_rec.app_of_list $ params ++ pds.map pred_predata.pred_g ++ [C] ++ rules,
-        apply $ const (pd.pred.const_name ++ "destruct") u_params',
+        apply $ func_rec.app_of_list $ params ++ pds.map coind_pred.pred_g ++ [C] ++ rules,
+        apply $ pd.destruct,
         exact h),
     set_basic_attribute `elab_as_eliminator cases_on.const_name),
 
+  /- prove `corec_on` rules -/
+  pds.mmap (λpd:coind_pred, do
+    rules ← pds.mmap (λpd, do
+      intros ← pd.intros.mmap (λr:coind_rule, do
+        eqs ← (list.zip pd.locals r.insts).mmap (λ⟨l, i⟩, do
+          sort u ← infer_type l.local_type,
+          return $ (const `eq [u] : expr) l.local_type l i),
+        mk_exists_lst r.loc_args $ mk_and_lst eqs),
+      mk_local_def (mk_simple_name $ "h_" ++ pd.pd_name.last_string) $
+        ((pd.f₁.app_of_list pd.locals).imp (mk_or_lst intros)).pis pd.locals),
+    h ← mk_local_def `h $ pd.f₁.app_of_list pd.locals,
+    pd.add_theorem (pd.pred.const_name ++ "corec_on")
+      (pd.pred_g.app_of_list pd.locals) (fs₁ ++ pd.impl_locals ++ [h] ++ rules)
+      (do
+        apply $ pd.corec_functional.app_of_list fs₁,
+        (pds.zip rules).mmap (λ⟨pd, hr⟩, solve1 $ do
+          ls ← intro_lst $ pd.locals.map local_pp_name,
+          h' ← intro `h,
+          h' ← note `h' none $ hr.app_of_list ls h',
+          match pd.intros.length with
+          | 0     := induction h' >> skip -- h' : false
+          | (n+1) := do
+            hs ← elim_gen_sum n h',
+            (hs.zip pd.intros).mmap (λ⟨h, r⟩, solve1 $ do
+              (as, h)    ← elim_gen_prod (r.args.length) h [],
+              (eqs, eq') ← elim_gen_prod (pd.locals.length - 1) h [],
+              let eqs := eqs ++ [eq'],
+              eqs.mmap subst,
+              apply ((const r.func_nm u_params).app_of_list $ params ++ fs₁ ++ as)),
+            skip
+          end),
+        exact h)),
+  
   /- prove constructors -/
-  pds.mmap (λpd:pred_predata, do
-    pd.intros.mmap (λ⟨nr, t⟩, do
-      let t := t.instantiate_locals $ pds.map $ λpd:pred_predata, (pd.pd_name, pd.pred_g),
-      pd.add_theorem nr t [] $ do
-        (name.mk_string sub p) ← return nr,
-        bs ← intros,
-        apply $ pd.construct.app_of_list $ params,
-        exact $ (const ((p ++ "functional") ++ sub) u_params').app_of_list $
-          params ++ pds.map pred_predata.pred_g ++ bs)),
+  pds.mmap (λpd:coind_pred, pd.intros.mmap (λr,
+    pd.add_theorem r.orig_nm r.type [] $ do
+      bs ← intros,
+      apply $ pd.construct,
+      exact $ (const r.func_nm u_params).app_of_list $ params ++ pds.map coind_pred.pred_g ++ bs)),
 
-  pds.mmap (λpd:pred_predata, do
-    set_basic_attribute `irreducible pd.pd_name),
+  pds.mmap (λpd:coind_pred, set_basic_attribute `irreducible pd.pd_name),
 
   try triv -- we setup a trivial goal for the tactic framework
 
